theories/Helpers.v
@@ -1,6 +1,8 @@
 (* Copyright 2025 Bloomberg Finance L.P. *)
 (* Distributed under the terms of the Apache 2.0 license. *)
 
+(** Small dependent-list and proof-transport helpers used across the library. *)
+
 Require Import Corelib.Relations.Relation_Definitions.
 From Stdlib Require Import List.
 
@@ -13,7 +15,7 @@ Notation "x .2" := (proj2_sig x) (at level 1, left associativity, format "x .2")
 
 Ltac inv x := inversion x; subst; clear x.
 
-(* The eta law for the [sig] inductive type. *)
+(** The eta law for the [sig] inductive type. *)
 Lemma sig_eta :
   forall {A : Type} (P : A -> Prop) (p : sig P), p = (p.1; p.2).
 Proof.
@@ -21,7 +23,7 @@ Proof.
   destruct p. simpl. auto.
 Qed.
 
-(* Function application at the [Forall] level. *)
+(** Function application at the [Forall] level. *)
 Lemma Forall_appl :
   forall {A B : Type}
          (P : A -> B -> Prop)
@@ -35,7 +37,7 @@ Proof.
   eapply Forall_cons; auto.
 Qed.
 
-(* Modus ponens at the [Forall] level. *)
+(** Modus ponens at the [Forall] level. *)
 Lemma Forall_mp :
   forall {A : Type}
          (P Q : A -> Prop)
@@ -51,7 +53,7 @@ Proof.
   eapply Forall_cons; auto.
 Qed.
 
-(* Convert a list of [P]-satisfying dependent pairs (i.e. [sig]),
+(** Convert a list of [P]-satisfying dependent pairs (i.e. [sig]),
    into a dependent pair of a [list] and that the entire list satisfies [P]. *)
 Fixpoint unite
   {A : Type} {P : A -> Prop} (l : list {a : A | P a}) : {l : list A | Forall P l}.
@@ -65,7 +67,7 @@ Proof.
   exact (xs'.2).
 Defined.
 
-(* Same thing as [distribute], but this auxiliary function takes
+(** Same thing as [distribute], but this auxiliary function takes
    the [list] and the proof separately so that
    it can do structural recursion on the list. *)
 Fixpoint zip_proofs
@@ -77,14 +79,14 @@ Proof.
   * refine ((x; _) :: @zip_proofs A P xs _); inversion pf; auto.
 Defined.
 
-(* Convert a [list] and a proof that all the elements of the list satisfy [P],
+(** Convert a [list] and a proof that all the elements of the list satisfy [P],
    into a list of dependent pairs where each element satisfies [P]. *)
 Definition distribute
   {A : Type} {P : A -> Prop}
   (lpf : {l : list A | Forall P l}) : list {a : A | P a} :=
   zip_proofs lpf.1 lpf.2.
 
-(* To show that round trip between distribute and unite preserves the elements. *)
+(** To show that round trip between distribute and unite preserves the elements. *)
 Lemma distribute_unite :
   forall
     {A : Type} {P : A -> Prop} (l : list {a : A | P a}),
@@ -98,7 +100,7 @@ Proof.
   auto.
 Qed.
 
-(* To show that round trip between distribute and unite preserves the elements. *)
+(** To show that round trip between distribute and unite preserves the elements. *)
 Lemma unite_distribute :
   forall
     {A : Type} {P : A -> Prop} (l : list A) (pf : Forall P l),
@@ -109,7 +111,7 @@ Proof.
   induction l; simpl; f_equal; auto.
 Qed.
 
-(* If the dependent pair (a; p) is in the [distribute]d list,
+(** If the dependent pair (a; p) is in the [distribute]d list,
    then [a] was in the first projection of [l]. *)
 Lemma In_distribute :
   forall
