theories/Trees.v
@@ -1,6 +1,8 @@
 (* Copyright 2025 Bloomberg Finance L.P. *)
 (* Distributed under the terms of the Apache 2.0 license. *)
 
+(** Finite rose trees and structural lemmas for game-tree algorithms. *)
+
 Require Import Corelib.Program.Wf.
 Require Import Corelib.Relations.Relation_Definitions.
 From Stdlib Require Import List.
@@ -13,7 +15,7 @@ Require Import GameTrees.Relations.
 
 Import ListNotations.
 
-(* A rose tree. *)
+(** A rose tree. *)
 Inductive tree (A : Type) : Type :=
 | node : A -> list (tree A) -> tree A.
 
@@ -36,7 +38,7 @@ Fixpoint size_tree {A : Type} (t : tree A) : nat :=
   | node a f => 1 + list_sum (map size_tree f)
   end.
 
-(* Returns the elements of a tree in pre-order. *)
+(** Returns the elements of a tree in pre-order. *)
 Fixpoint flatten_tree {A : Type} (t : tree A) : list A :=
   match t with
   | node a f => a :: concat (map flatten_tree f)
@@ -59,7 +61,7 @@ Definition singleton_forest {A : Type} (a : A) : forest A := [node a []].
 Definition forest_of_list {A : Type} (l : list A) : forest A :=
   map singleton_tree l.
 
-(* Take the [height]-many levels from the tree *)
+(** Take the [height]-many levels from the tree *)
 Fixpoint take_tree {A : Type} (height : nat) (t : tree A) : tree A :=
   match t with
   | node a f =>
@@ -81,7 +83,7 @@ Fixpoint leaves {A : Type} (t : tree A) : list A :=
   | node _ f => concat (map leaves f)
   end.
 
-(* A [tree] is monotonic w.r.t. [R] if each node respects an incoming bound:
+(** A [tree] is monotonic w.r.t. [R] if each node respects an incoming bound:
    [None] = no constraint; [Some b] requires the node label [a] to satisfy [R a b].
    The children are checked with bound [Some a]. *)
 Inductive monotonic_tree {A : Type} (R : relation A)
@@ -96,13 +98,13 @@ Inductive monotonic_tree {A : Type} (R : relation A)
       Forall (monotonic_tree R (Some a)) f ->
       monotonic_tree R (Some b) (node a f).
 
-(* A forest is monotonic when every tree in it is monotonic under the same bound. *)
+(** A forest is monotonic when every tree in it is monotonic under the same bound. *)
 Definition monotonic_forest
           {A : Type} (R : relation A)
           (bound : option A) (f : forest A) : Prop :=
   Forall (monotonic_tree R bound) f.
 
-(* A better induction principle for [tree],
+(** A better induction principle for [tree],
    since [tree_ind] does not specify that [P] holds for the subtrees. *)
 Fixpoint tree_forall_ind
     (A : Type) (P : tree A -> Prop)
@@ -115,7 +117,7 @@ Fixpoint tree_forall_ind
            (fun x xs IHxs => Forall_cons x (tree_forall_ind A P tpf x) IHxs) f)
   end.
 
-(* Mapping node labels through a [monotone] function [g] preserves monotonicity:
+(** Mapping node labels through a [monotone] function [g] preserves monotonicity:
    an [R1]-monotone [tree] becomes [R2]-monotone, under the mapped [bound]. *)
 Lemma map_tree_monotonic :
   forall {A B : Type}
@@ -185,7 +187,7 @@ Proof.
   repeat (constructor; auto).
 Qed.
 
-(* A predicate on [tree]s, under which all nodes in a [tree] satisfy [P]. *)
+(** A predicate on [tree]s, under which all nodes in a [tree] satisfy [P]. *)
 Inductive Forall_nodes {A : Type} (P : A -> Prop) : tree A -> Prop :=
 | Forall_nodes_node : forall a f, P a -> Forall (Forall_nodes P) f -> Forall_nodes P (node a f).
 
@@ -259,7 +261,7 @@ Proof.
   inversion H2; subst; auto.
 Qed.
 
-(* A predicate on [tree]s, under which a particular node label [a] occurs in the [tree].
+(** A predicate on [tree]s, under which a particular node label [a] occurs in the [tree].
    Can be compared to [In] for [list]s. *)
 Inductive In_tree {A : Type} (a : A) : tree A -> Prop :=
 | In_this : forall f, In_tree a (node a f)
@@ -268,7 +270,7 @@ Inductive In_tree {A : Type} (a : A) : tree A -> Prop :=
 Definition In_forest {A : Type} (a : A) (f : forest A) : Prop :=
   Exists (fun t => In_tree a t) f.
 
-(* The [Forall_nodes] and [In_tree] counterpart of [Forall_forall]. *)
+(** The [Forall_nodes] and [In_tree] counterpart of [Forall_forall]. *)
 Lemma Forall_nodes_In_tree :
   forall {A : Type} (P : A -> Prop) (t : tree A),
     Forall_nodes P t <-> (forall (x : A), In_tree x t -> P x).
@@ -304,39 +306,39 @@ Proof.
       right; auto. } }
 Qed.
 
-(* [P] holds at the current node and recursively for every sub[tree];
+(** [P] holds at the current node and recursively for every sub[tree];
    equivalently, [P] holds at every node of the tree.
    Can be compared to AG P in CTL. *)
 Inductive Forall_subtrees {A : Type} (P : tree A -> Prop) : tree A -> Prop :=
 | Forall_subtrees_node : forall a f, P (node a f) -> Forall (Forall_subtrees P) f -> Forall_subtrees P (node a f).
 
-(* Either [P] holds here or in some descendant;
+(** Either [P] holds here or in some descendant;
    i.e., there exists a node along some branch where [P] holds.
    Can be compared to EF P in CTL. *)
 Inductive Exists_subtree {A : Type} (P : tree A -> Prop) : tree A -> Prop :=
 | Exists_subtree_here : forall a f, P (node a f) -> Exists_subtree P (node a f)
 | Exists_subtree_there : forall a f, Exists (Exists_subtree P) f -> Exists_subtree P (node a f).
 
-(* Either [P] holds here or all children continue to satisfy it;
+(** Either [P] holds here or all children continue to satisfy it;
    i.e., along every branch, [P] eventually holds.
    Can be compared to AF P in CTL. *)
 Inductive Exists_all_paths {A : Type} (P : tree A -> Prop) : tree A -> Prop :=
 | Exists_all_paths_here : forall a f, P (node a f) -> Exists_all_paths P (node a f)
 | Exists_all_paths_there : forall a f, Forall (Exists_all_paths P) f -> Exists_all_paths P (node a f).
 
-(* On every path, nodes satisfy [P1] up to the first node where [P2] holds (possibly here).
+(** On every path, nodes satisfy [P1] up to the first node where [P2] holds (possibly here).
    Can be compared to A[P1 U P2] in CTL. *)
 Inductive AllUntil {A : Type} (P1 P2 : tree A -> Prop) : tree A -> Prop :=
 | AllUntil_here : forall a f, P2 (node a f) -> AllUntil P1 P2 (node a f)
 | AllUntil_there : forall a f, P1 (node a f) -> Forall (AllUntil P1 P2) f -> AllUntil P1 P2 (node a f).
 
-(* There exists a path where nodes satisfy [P1] until a node where [P2] holds (possibly here).
+(** There exists a path where nodes satisfy [P1] until a node where [P2] holds (possibly here).
    Can be compared to E[P1 U P2] in CTL. *)
 Inductive ExistsUntil {A : Type} (P1 P2 : tree A -> Prop) : tree A -> Prop :=
 | ExistsUntil_here : forall a f, P2 (node a f) -> ExistsUntil P1 P2 (node a f)
 | ExistsUntil_there : forall a f, P1 (node a f) -> Exists (ExistsUntil P1 P2) f -> ExistsUntil P1 P2 (node a f).
 
-(* Unfolding of a tree with an explicit [Acc] argument.
+(** Unfolding of a tree with an explicit [Acc] argument.
    This is the auxiliary function to [unfold_tree]. *)
 Fixpoint unfold_tree_aux
     {A : Type}
@@ -351,7 +353,7 @@ Fixpoint unfold_tree_aux
                    (distribute (next init)))
   end.
 
-(* The entry point of unfolding of a tree.
+(** The entry point of unfolding of a tree.
    This function takes a well-founded relation,
    and calls the well-foundedness proof to generate an [Acc]
    to call the auxiliary function with. *)
@@ -364,7 +366,7 @@ Definition unfold_tree
   : tree A :=
   unfold_tree_aux R next init (wellfounded init).
 
-(* If [P] holds at [init] and is preserved from any [a] to all its [R]-smaller successors,
+(** If [P] holds at [init] and is preserved from any [a] to all its [R]-smaller successors,
    then every node in [unfold_tree_aux R next init acc] satisfies [P]. *)
 Fixpoint Forall_unfold_tree_aux
     {A : Type}
@@ -390,7 +392,7 @@ Proof.
   auto.
 Qed.
 
-(* If [P] holds at [init] and is preserved from any [a] to all its [R]-smaller successors,
+(** If [P] holds at [init] and is preserved from any [a] to all its [R]-smaller successors,
    then every node in [unfold_tree R next init] satisfies [P]. *)
 Lemma Forall_unfold_tree :
   forall
@@ -408,7 +410,7 @@ Proof.
   eapply Forall_unfold_tree_aux; auto.
 Qed.
 
-(* The result of [unfold_tree_aux] is independent of the [Acc] argument. *)
+(** The result of [unfold_tree_aux] is independent of the [Acc] argument. *)
 Fixpoint unfold_tree_aux_same
     {A : Type}
     (R : relation A)
@@ -427,7 +429,7 @@ Proof.
   eapply unfold_tree_aux_same.
 Qed.
 
-(* A relation between two game states
+(** A relation between two game states
    where the game state [y] occurs after the game state [x]. *)
 Definition step
            {A : Type} {R : relation A}
@@ -435,7 +437,7 @@ Definition step
            (x y : A) : Prop :=
   In y (next x).1.
 
-(* There is a sequence of steps from x to y in zero or more steps,
+(** There is a sequence of steps from x to y in zero or more steps,
    where a one-step edge is "y appears in [next] x". *)
 Definition reachable
            {A : Type} {R : relation A}
@@ -443,14 +445,14 @@ Definition reachable
            : A -> A -> Prop :=
   clos_refl_trans _ (step next).
 
-(* Same as [reachable], but the transitive closure is left-stepping. *)
+(** Same as [reachable], but the transitive closure is left-stepping. *)
 Definition reachable_1n
            {A : Type} {R : relation A}
            (next : forall (a : A), {l : list A | Forall (fun x => R x a) l })
            : A -> A -> Prop :=
   clos_refl_trans_1n _ (fun (x y : A) => In y (next x).1).
 
-(* The soundness proof for [unfold_tree_aux]. *)
+(** The soundness proof for [unfold_tree_aux]. *)
 Fixpoint unfold_tree_aux_sound
     {A : Type}
     (R : relation A)
@@ -478,7 +480,7 @@ Proof.
   eapply (unfold_tree_aux_sound A R next x _ y i''').
 Qed.
 
-(* If a state is the unfolded game tree,
+(** If a state is the unfolded game tree,
    then that state must be [reachable] in a game from the initial state. *)
 Theorem unfold_tree_sound :
   forall
@@ -495,7 +497,7 @@ Proof.
   eapply unfold_tree_aux_sound; eauto.
 Qed.
 
-(* An explicit unfolding of a call to [unfold_tree] is equal to the original. *)
+(** An explicit unfolding of a call to [unfold_tree] is equal to the original. *)
 Lemma unfold_tree_unwrap :
   forall
     {A : Type}
@@ -522,7 +524,7 @@ Proof.
   Transparent unfold_tree_aux.
 Qed.
 
-(* Any game state left-steppingly [reachable] from the initial state
+(** Any game state left-steppingly [reachable] from the initial state
    must be in the unfolded game tree. *)
 Lemma unfold_tree_complete_1n :
   forall
@@ -547,7 +549,7 @@ Proof.
   eapply in_map; eauto.
 Qed.
 
-(* Any game state [reachable] from the initial state
+(** Any game state [reachable] from the initial state
    must be in the unfolded game tree. *)
 Theorem unfold_tree_complete :
   forall
